Remove gFunctorList and use gFunctors everywhere.
This makes stuff more uniform and also removes the need for the [inGFs]
type class. Instead, there is now a type class [subG Σ1 Σ2] which expresses
that a list of functors [Σ1] is contained in [Σ2].

program_logic/ghost_ownership.v
@@ -1,33 +1,60 @@
-From iris.program_logic Require Export global_functor.
+From iris.program_logic Require Export model.
 From iris.algebra Require Import iprod gmap.
 Import uPred.
 
+(** The class [inG Σ A] expresses that the CMRA [A] is in the list of functors
+[Σ]. This class is similar to the [subG] class, but written down in terms of
+individual CMRAs instead of lists of CMRA functors. This additional class is
+needed because Coq is otherwise unable to solve type class constraints due to
+higher-order unification problems. *)
+Class inG (Σ : gFunctors) (A : cmraT) :=
+  InG { inG_id : gid Σ; inG_prf : A = Σ inG_id (iPreProp Σ) }.
+Arguments inG_id {_ _} _.
+
+Lemma subG_inG Σ (F : gFunctor) : subG F Σ → inG Σ (F (iPreProp Σ)).
+Proof. move=> /(_ 0%fin) /= [j ->]. by exists j. Qed.
+
+(** * Definition of the connective [own] *)
+Definition iRes_singleton `{i : inG Σ A} (γ : gname) (a : A) : iResUR Σ :=
+  iprod_singleton (inG_id i) {[ γ := cmra_transport inG_prf a ]}.
+Instance: Params (@iRes_singleton) 4.
+
 Definition own_def `{inG Σ A} (γ : gname) (a : A) : iProp Σ :=
-  uPred_ownM (to_iRes γ a).
+  uPred_ownM (iRes_singleton γ a).
 Definition own_aux : { x | x = @own_def }. by eexists. Qed.
 Definition own {Σ A i} := proj1_sig own_aux Σ A i.
 Definition own_eq : @own = @own_def := proj2_sig own_aux.
 Instance: Params (@own) 4.
 Typeclasses Opaque own.
 
-(** Properties about ghost ownership *)
+(** * Properties about ghost ownership *)
 Section global.
 Context `{i : inG Σ A}.
 Implicit Types a : A.
 
-(** * Properties of own *)
+(** ** Properties of [iRes_singleton] *)
+Global Instance iRes_singleton_ne γ n :
+  Proper (dist n ==> dist n) (@iRes_singleton Σ A _ γ).
+Proof. by intros a a' Ha; apply iprod_singleton_ne; rewrite Ha. Qed.
+Lemma iRes_singleton_op γ a1 a2 :
+  iRes_singleton γ (a1 ⋅ a2) ≡ iRes_singleton γ a1 ⋅ iRes_singleton γ a2.
+Proof.
+  by rewrite /iRes_singleton iprod_op_singleton op_singleton cmra_transport_op.
+Qed.
+
+(** ** Properties of [own] *)
 Global Instance own_ne γ n : Proper (dist n ==> dist n) (@own Σ A _ γ).
 Proof. rewrite !own_eq. solve_proper. Qed.
 Global Instance own_proper γ :
   Proper ((≡) ==> (⊣⊢)) (@own Σ A _ γ) := ne_proper _.
 
 Lemma own_op γ a1 a2 : own γ (a1 ⋅ a2) ⊣⊢ own γ a1 ★ own γ a2.
-Proof. by rewrite !own_eq /own_def -ownM_op to_iRes_op. Qed.
+Proof. by rewrite !own_eq /own_def -ownM_op iRes_singleton_op. Qed.
 Global Instance own_mono γ : Proper (flip (≼) ==> (⊢)) (@own Σ A _ γ).
 Proof. move=>a b [c ->]. rewrite own_op. eauto with I. Qed.
 Lemma own_valid γ a : own γ a ⊢ ✓ a.
 Proof.
-  rewrite !own_eq /own_def ownM_valid /to_iRes.
+  rewrite !own_eq /own_def ownM_valid /iRes_singleton.
   rewrite iprod_validI (forall_elim (inG_id i)) iprod_lookup_singleton.
   rewrite gmap_validI (forall_elim γ) lookup_singleton option_validI.
   (* implicit arguments differ a bit *)
@@ -42,13 +69,14 @@ Proof. rewrite !own_eq /own_def; apply _. Qed.
 Global Instance own_core_persistent γ a : Persistent a → PersistentP (own γ a).
 Proof. rewrite !own_eq /own_def; apply _. Qed.
 
+(** ** Allocation *)
 (* TODO: This also holds if we just have ✓ a at the current step-idx, as Iris
    assertion. However, the map_updateP_alloc does not suffice to show this. *)
 Lemma own_alloc_strong a (G : gset gname) :
   ✓ a → True =r=> ∃ γ, ■ (γ ∉ G) ∧ own γ a.
 Proof.
   intros Ha.
-  rewrite -(rvs_mono (∃ m, ■ (∃ γ, γ ∉ G ∧ m = to_iRes γ a) ∧ uPred_ownM m)%I).
+  rewrite -(rvs_mono (∃ m, ■ (∃ γ, γ ∉ G ∧ m = iRes_singleton γ a) ∧ uPred_ownM m)%I).
   - rewrite ownM_empty.
     eapply rvs_ownM_updateP, (iprod_singleton_updateP_empty (inG_id i));
       first (eapply alloc_updateP_strong', cmra_transport_valid, Ha);
@@ -62,10 +90,11 @@ Proof.
   apply rvs_mono, exist_mono=>?. eauto with I.
 Qed.
 
+(** ** Frame preserving updates *)
 Lemma own_updateP P γ a : a ~~>: P → own γ a =r=> ∃ a', ■ P a' ∧ own γ a'.
 Proof.
   intros Ha. rewrite !own_eq.
-  rewrite -(rvs_mono (∃ m, ■ (∃ a', m = to_iRes γ a' ∧ P a') ∧ uPred_ownM m)%I).
+  rewrite -(rvs_mono (∃ m, ■ (∃ a', m = iRes_singleton γ a' ∧ P a') ∧ uPred_ownM m)%I).
   - eapply rvs_ownM_updateP, iprod_singleton_updateP;
       first by (eapply singleton_updateP', cmra_transport_updateP', Ha).
     naive_solver.
