heap_lang/lib/lock.v
@@ -14,9 +14,10 @@ Global Opaque newlock acquire release.
 (** The CMRA we need. *)
 (* Not bundling heapG, as it may be shared with other users. *)
 Class lockG Σ := LockG { lock_tokG :> inG Σ (exclR unitC) }.
-Definition lockGF : gFunctorList := [GFunctor (constRF (exclR unitC))].
-Instance inGF_lockG `{H : inGFs Σ lockGF} : lockG Σ.
-Proof. destruct H. split. apply: inGF_inG. Qed.
+
+Definition lockΣ : gFunctors := #[GFunctor (constRF (exclR unitC))].
+Instance subG_lockΣ {Σ} : subG lockΣ Σ → lockG Σ.
+Proof. intros [?%subG_inG _]%subG_inv. split; apply _. Qed.
 
 Section proof.
 Context `{!heapG Σ, !lockG Σ} (N : namespace).
