tests/counter.v
@@ -72,9 +72,9 @@ Section M.
 End M.
 
 Class counterG Σ := CounterG { counter_tokG :> inG Σ M_UR }.
-Definition counterGF : gFunctorList := [GFunctor (constRF M_UR)].
-Instance inGF_counterG `{H : inGFs Σ counterGF} : counterG Σ.
-Proof. destruct H. split. apply: inGF_inG. Qed.
+Definition counterΣ : gFunctors := #[GFunctor (constRF M_UR)].
+Instance subG_counterΣ {Σ} : subG counterΣ Σ → counterG Σ.
+Proof. intros [?%subG_inG _]%subG_inv. split; apply _. Qed.
 
 Section proof.
 Context `{!heapG Σ, !counterG Σ}.
